\documentclass{article}

\usepackage{amsmath}

\begin{document}

\title{Solution of Geometric Brownian Motion SDE}
\maketitle

\section{The SDE}

Geometric Brownian motion SDE:
\begin{equation}
  \begin{aligned}
    \frac{dS(t)}{S(t)} & = \mu dt + \sigma \sqrt{dt} z \\
      z & \sim \mathcal{N}(0,1)
  \end{aligned}
\end{equation}

Raise to square:
\begin{equation}
  \begin{aligned}
    {dS(t)}^2 & = {(\mu S(t) dt + \sigma S(t) \sqrt{dt} z)}^2 \\
    & = {\mu}^2 {S(t)}^2 {dt}^2 + 2 \mu \sigma {S(t)}^2 dt \sqrt{dt} + {\sigma}^2 {S(t)}^2 {(\sqrt{dt})}^2 {z}^2
  \end{aligned}
\end{equation}

When ${dt \to 0}$ we have $dt^2 = 0$ and $dt \sqrt{dt} = 0$. Also since $z \sim \mathcal{N}(0,1)$ one can verify that on average $z^2 = 1$.

Therefore:
\begin{equation}
  {dS(t)}^2 = {\sigma}^2 {S(t)}^2 dt
\end{equation}

\section{Stochastic Integrals}

Take the following integral:
\begin{equation}
  \begin{aligned}
   I & = \int_{0}^{t} dW(t) \\
     & = \int_{0}^{t} \sigma \sqrt{dt} z \\
     z & \sim \mathcal{N}(0,1)
  \end{aligned}
\end{equation}

Dividing the interval $\left[ 0, t \right]$ into $n \to \infty$ equal subintervals of equal size $dt$ we have:
\begin{equation}
  \begin{aligned}
   I & = \sum_{i=0}^{n} \left( \sigma \sqrt{dt} z_{i} \right) \\
     & = \sigma \sqrt{dt} \sum_{i=0}^{n} z_{i}
  \end{aligned}
\end{equation}

Since we are adding $n$ normal distributed random variables of mean zero and variance $\sigma^2 dt$, their sum will be still a normal distributed random variable of mean zero and variance $n \sigma^2 dt$. But $n dt = t$ so finally we get the variance $\sigma^t t$ so the deviation $\sigma \sqrt{t}$. Therefore:

\begin{equation}
  \begin{aligned}
   I & = W(t) \\
   \int_{0}^{t} \sigma \sqrt{dt} z & = \sigma \sqrt{t} z \\
     z & \sim \mathcal{N}(0,1)
  \end{aligned}
\end{equation}

\section{The solution}

Take the function $f(S, t) = \ln{S(t)}$. We have it's Taylor series expansion:

\begin{equation}
  \begin{aligned}
    df(S, t) & \approx \frac{\partial f}{\partial t} dt + \frac{\partial f}{\partial S} dS + \frac{1}{2} \frac{{\partial}^2 f}{\partial t^2} {dt}^2 +
               \frac{{\partial}^2 f}{\partial t \partial S} dt dS + \frac{1}{2} \frac{{\partial}^2 f}{\partial S^2} {dS}^2
  \end{aligned}
\end{equation}

We then have the partial derivatives:
\begin{equation}
  \begin{aligned}
    \frac{\partial \ln{S(t)}}{\partial t} & = 0 \\
    \frac{\partial \ln{S(t)}}{\partial S} & = \frac{1}{S(t)} \\
    \frac{{\partial}^2 \ln{S(t)}}{\partial t^2} & = 0 \\
    \frac{{\partial}^2 \ln{S(t)}}{\partial S \partial t} & = 0 \\
    \frac{{\partial}^2 \ln{S(t)}}{\partial S^2} & = - \frac{1}{{S(t)}^2}
  \end{aligned}
\end{equation}

Replacing in the We Taylor series expansion we get:

\begin{equation}
  \begin{aligned}
    d \left( \ln{S(t)} \right) & \approx \frac{1}{S(t)} dS(t) - \frac{1}{S(t)^2} {dS(t)}^2
  \end{aligned}
\end{equation}

By equation (3) we then have:

\begin{equation}
  \begin{aligned}
    d \left( \ln{S(t)} \right) & \approx \frac{dS(t)}{S(t)} - \frac{1}{2} \frac{{\sigma}^2 {S(t)}^2}{{S(t)}^2} dt \Leftrightarrow \\
    d \left( \ln{S(t)} \right) & = \frac{dS(t)}{S(t)} - \frac{{\sigma}^2 }{2} dt
  \end{aligned}
\end{equation}

Replacing from (1) $\frac{dS(t)}{S(t)}$ we get:

\begin{equation}
  \begin{aligned}
    d \left( \ln{S(t)} \right) & = \mu dt + \sigma \sqrt{dt} z - \frac{{\sigma}^2 }{2} dt \Leftrightarrow \\
    d \left( \ln{S(t)} \right) & = \left( \mu - \frac{{\sigma}^2 }{2} \right) dt + \sigma \sqrt{dt} z \\
    d \left( \ln{S(t)} \right) & = \left( \mu - \frac{{\sigma}^2 }{2} \right) dt + \sigma dW(t) \\
  \end{aligned}
\end{equation}

Where we have denoted the differential of the Weiner process $dW(t) \approx \sqrt{dt} z$.

Integrating:
\begin{equation}
  \begin{aligned}
    \int_{0}^{t} d \left( \ln{S(t)} \right) & = \int_{0}^{t} \left( \mu - \frac{{\sigma}^2 }{2} \right) dt + \int_{0}^{t} \sigma dW(t) \Rightarrow \\
    \ln{S(t)} \Big|_{0}^{t} & = \left( \mu - \frac{{\sigma}^2 }{2} \right) t \Big|_{0}^{t} + \sigma W(t) \Big|_{0}^{t} \Leftrightarrow \\
    \ln{S(t)} - \ln{S(0)} & = \left( \mu - \frac{{\sigma}^2 }{2} \right) t + \sigma W(t) \Leftrightarrow \\
    \ln{\frac{S(t)}{S(0)}} & = \left( \mu - \frac{{\sigma}^2 }{2} \right) t + \sigma \sqrt{t} z \\
    z & \sim \mathcal{N}(0,1)
  \end{aligned}
\end{equation}

Taking the exponential:
\begin{equation}
  \begin{aligned}
    e^{\ln{\frac{S(t)}{S(0)}}} & = e^{\left( \mu - \frac{{\sigma}^2 }{2} \right) t + \sigma \sqrt{t} z} \Rightarrow \\
    \frac{S(t)}{S(0)} & = e^{\left( \mu - \frac{{\sigma}^2 }{2} \right) t + \sigma \sqrt{t} z}
  \end{aligned}
\end{equation}

Which finally gives the solution:
\begin{equation}
  \begin{aligned}
    S(t) & = S(0) e^{\left( \mu - \frac{{\sigma}^2 }{2} \right) t + \sigma \sqrt{t} z} \\
    z & \sim \mathcal{N}(0,1)
  \end{aligned}
\end{equation}

\end{document}
